
\usepackage[active,tightpage,auctex]{preview}

\setlength{\textwidth}{0.6\paperwidth}

\begin{document}

\setlength\abovedisplayskip{0pt} % Remove padding before equation environments.


\begin{preview}
\setcounter{equation}{0}%
\begin{align}
  &E[E[Y|X]] =E[g(x)] = \int_{IR} g(x) f_x(x) \mathrm{d} x, g(x) = E[Y|X=x]\\
  &\Rightarrow \int_{IR}[\int_{IR} y f_{Y|X}(y|x) \mathrm{d}y] f_X(x)\mathrm{d}x\\
  &=\int_{IR}[\int_{IR}yf_{Y|X}(y|x)f_X(x)\mathrm{d}y]\mathrm{d}x\\
  &=\int_{IR}\int_{IR} yf(x, y)\mathrm{d}y \mathrm{d}x\\
  &=E[Y].
\end{align}

\end{preview}

\begin{preview}
\setcounter{equation}{0}%
\begin{align}
  D(X|Y = y) = E\{[X - E(X|Y=y)]^2|Y=y\}
\end{align}

\end{preview}

\begin{preview}
\setcounter{equation}{0}%
\(E(Y|X=x) = \mu(x), E(X|Y=y) = \delta(y)\)
\end{preview}

\begin{preview}
\setcounter{equation}{0}%
\begin{align}
f_Z(z) = \int_{IR}f(x, z-x)dz
\end{align}

\end{preview}

\begin{preview}
\setcounter{equation}{0}%
\begin{align}
P\left\{\frac{\sum^n_{i=1} X_i - n\mu}{\sqrt{n\sigma^2}}\leq x \right\} \rightarrow \Phi(x)
\end{align}

\end{preview}

\begin{preview}
\setcounter{equation}{0}%
\(X, Y\)
\end{preview}

\begin{preview}
\setcounter{equation}{0}%
\(Z = X + jY\)
\end{preview}

\begin{preview}
\setcounter{equation}{0}%
\begin{align}
  E(Z) = E(X) + j E(Y), j = \sqrt{-1}.
\end{align}

\end{preview}

\begin{preview}
\setcounter{equation}{0}%
\begin{align}
  E(e^{jtX}) &= E(\cos{t}X) + jE(\sin{t}X)\\
&=\int^{+\infty}_{-\infty} \cos{tx}  \mathrm{d}F(x) + j\int^{+\infty}_{-\infty} \sin{tx}\mathrm{d}F(x)\\
&=\int^{+\infty}_{-\infty} e^{jtx}\mathrm{d}F(x)
\end{align}

\end{preview}

\begin{preview}
\setcounter{equation}{0}%
\(\forall t \in R, \cos{t}x, \sin{t}x\)
\end{preview}

\begin{preview}
\setcounter{equation}{0}%
\(E(e^{jtX})\)
\end{preview}

\begin{preview}
\setcounter{equation}{0}%
\(E(e^{jtX})\)
\end{preview}

\begin{preview}
\setcounter{equation}{0}%
\(X\)
\end{preview}

\begin{preview}
\setcounter{equation}{0}%
\((\Omega, \mathcal{F}, P)\)
\end{preview}

\begin{preview}
\setcounter{equation}{0}%
\begin{align}
  \varphi(t) = E(e^{jtX}) = \int^{+\infty}_{-\infty} e^{jtX} \mathrm{d}F(x), t\in R
\end{align}

\end{preview}

\begin{preview}
\setcounter{equation}{0}%
\(X\)
\end{preview}

\begin{preview}
\setcounter{equation}{0}%
\begin{align}P\{X = c\} = 1, \varphi(t) = E(e^{jtc}) = e^{jtc}, t \in R\end{align}

\end{preview}

\begin{preview}
\setcounter{equation}{0}%
\begin{align}
\varphi(t) &= e^{jt \cdot 0} (1-p) + e^{jt \cdot 1} p\\
&= 1 - p + pe^{jt} = q + pe^{jt}, t\in R
\end{align}

\end{preview}

\begin{preview}
\setcounter{equation}{0}%
\begin{align}
  \varphi(t) = (q + pe^{jt})^n, t \in R
\end{align}

\end{preview}

\begin{preview}
\setcounter{equation}{0}%
\begin{align}
  \varphi(t) = e^{\lambda(e^{jt} - 1)}, t \in R
\end{align}

\end{preview}

\begin{preview}
\setcounter{equation}{0}%
\begin{align}
  f(x) =
\left\{
\begin{aligned}
\lambda e^{- \lambda x}, & &x \geq 0;\\
0, & &x<0.\\
\end{aligned}
\right.{(\lambda > 0)}
\end{align}

\end{preview}

\begin{preview}
\setcounter{equation}{0}%
\begin{align}
  \varphi(t) &= \int^{+\infty}_{0} \lambda e^{jtx} e^{-\lambda x} \mathrm{d}x\\
&=\int^{+\infty}_{0} \lambda e^{-\lambda x} \cos{tx} \mathrm{d}x + j \lambda \int^{+\infty}_{0} e^{-\lambda x} \sin{tx} \mathrm{d}x\\
&= \lambda \frac{\lambda}{\lambda^2 + t^2} + j \lambda \frac{t}{\lambda^2 + t^2} = \left(1- \frac{jt}{\lambda}\right)^{-1}, t \in R.
\end{align}

\end{preview}

\begin{preview}
\setcounter{equation}{0}%
\(U[-a, a]\)
\end{preview}

\begin{preview}
\setcounter{equation}{0}%
\begin{align}
  \varphi(t) = \frac{\sin{at}}{at}, t \in R
\end{align}

\end{preview}

\begin{preview}
\setcounter{equation}{0}%
\(N(a, \sigma^2)\)
\end{preview}

\begin{preview}
\setcounter{equation}{0}%
\begin{align}
  \varphi(t) = e^{jat - \frac{1}{2}\sigma^2 t^2}, t\in R
\end{align}

\end{preview}

\begin{preview}
\setcounter{equation}{0}%
\(N(0, 1)\)
\end{preview}

\begin{preview}
\setcounter{equation}{0}%
\begin{align}
  \varphi(t) = e^{-\frac{1}{2}t^2}, t \in R.
\end{align}

\end{preview}

\begin{preview}
\setcounter{equation}{0}%
\(|\varphi(t)| \leq \varphi(0) = 1\)
\end{preview}

\begin{preview}
\setcounter{equation}{0}%
\(\overline{\varphi(t)} = \varphi (-t)\)
\end{preview}

\begin{preview}
\setcounter{equation}{0}%
\(\varphi_X(t)\)
\end{preview}

\begin{preview}
\setcounter{equation}{0}%
\(Y = a X + b\)
\end{preview}

\begin{preview}
\setcounter{equation}{0}%
\(  \varphi_Y(t) = e^{jbt} \varphi_X(at)\)
\end{preview}

\begin{preview}
\setcounter{equation}{0}%
\(\varphi(t)\)
\end{preview}

\begin{preview}
\setcounter{equation}{0}%
\(z_1, z_2, ..., z_n\)
\end{preview}

\begin{preview}
\setcounter{equation}{0}%
\(t_r \in R, r = 1, 2, ..., n\)
\end{preview}

\begin{preview}
\setcounter{equation}{0}%
\(\sum^n_{r=1} \sum^n_{s = 1} \varphi(t_r - t_s) z_r \overline{z_s} \geq 0\)
\end{preview}

\begin{preview}
\setcounter{equation}{0}%
\(\varphi(t)\)
\end{preview}

\begin{preview}
\setcounter{equation}{0}%
\(\varphi(t)\)
\end{preview}

\begin{preview}
\setcounter{equation}{0}%
\(\varphi^{(k)}(t)\)
\end{preview}

\begin{preview}
\setcounter{equation}{0}%
\begin{align}
  E(X^k) = j^{-k} \varphi^{(k)}(0), k \leq n.
\end{align}

\end{preview}

\begin{preview}
\setcounter{equation}{0}%
\begin{align}
E[(X-a)^k] =
\left\{
\begin{aligned}
&0, &k \% 2 == 1\\
&1 \cdot 3 \cdot 5 \cdot ...  \cdot (k-1)\sigma^k, & k \% 2 == 0\\
\end{aligned}
\right.
\end{align}

\end{preview}

\begin{preview}
\setcounter{equation}{0}%
\(F(x)\)
\end{preview}

\begin{preview}
\setcounter{equation}{0}%
\(\varphi(t)\)
\end{preview}

\begin{preview}
\setcounter{equation}{0}%
\(x_1, x_2(x_1 < x_2)\)
\end{preview}

\begin{preview}
\setcounter{equation}{0}%
\begin{align}
  \frac{F(x_2 + 0) + F(x_2 - 0)}{2} - \frac{F(x_1 + 0) + F(x_1 - 0)}{2} =\\ \lim_{T \rightarrow \infty} \frac{1}{2\pi} \int^T_{-T} \frac{e^{-jtx_1} - e^{-jtx_2}}{jt} \varphi(t) \mathrm{d}t.
\end{align}

\end{preview}

\begin{preview}
\setcounter{equation}{0}%
\(x_1, x_2\)
\end{preview}

\begin{preview}
\setcounter{equation}{0}%
\(F(x)\)
\end{preview}

\begin{preview}
\setcounter{equation}{0}%
\begin{align}
  F(x_2) - F(x_1) = \lim_{T \rightarrow \infty} \frac{1}{2\pi}\int^T_{-T} \frac{e^{-jtx_1} - e^{-jtx_2}}{jt}\varphi(t) \mathrm{d}t.
\end{align}

\end{preview}

\begin{preview}
\setcounter{equation}{0}%
\(x_2 = x, x_1 \rightarrow -\infty\)
\end{preview}

\begin{preview}
\setcounter{equation}{0}%
\begin{align}
  F(x) = \lim_{x_1 \rightarrow -\infty} \lim_{T \rightarrow +\infty} \frac{1}{2\pi} \int_{-T}^{T}\frac{e^{-jtx_1} - e^{-jtx}}{jt}\varphi(t) \mathrm{d}t.
\end{align}

\end{preview}

\begin{preview}
\setcounter{equation}{0}%
\(F_1(x)\)
\end{preview}

\begin{preview}
\setcounter{equation}{0}%
\(F_2(x)\)
\end{preview}

\begin{preview}
\setcounter{equation}{0}%
\(\varphi_1(t)\)
\end{preview}

\begin{preview}
\setcounter{equation}{0}%
\(\varphi_2(t)\)
\end{preview}

\begin{preview}
\setcounter{equation}{0}%
\(\xi\)
\end{preview}

\begin{preview}
\setcounter{equation}{0}%
\begin{align}
  f(x) = \frac{1}{\sqrt{2\pi} \sigma}e^{-\frac{(x-\mu)^2}{2\sigma^2}},x \in \mathbb{R}
\end{align}

\end{preview}

\begin{preview}
\setcounter{equation}{0}%
\(\xi\)
\end{preview}

\begin{preview}
\setcounter{equation}{0}%
\(\xi \sim N(\mu, \sigma^2)\)
\end{preview}

\begin{preview}
\setcounter{equation}{0}%
\(a \xi + b \sim N(a\mu + b, a^2 \sigma^2);\)
\end{preview}

\begin{preview}
\setcounter{equation}{0}%
   \begin{align}
   \xi \sim N(\mu, \sigma^2),
   \end{align}

\end{preview}

\begin{preview}
\setcounter{equation}{0}%
\(\xi \sim N(m_1, \sigma_1^2), \eta \sim N(m_2, \sigma_2^2)\)
\end{preview}

\begin{preview}
\setcounter{equation}{0}%
\( \xi + \eta \sim N(m_1 + m_2, \sigma_1^2 + \sigma_2^2).\)
\end{preview}

\begin{preview}
\setcounter{equation}{0}%
\begin{align}
  \varphi_{\xi+\eta}(t) = E[e^{jt(\xi+\eta)}] = &E[e^{jt\xi} \cdot e^{jt\eta}] \\
=&e^{jm_1t - \frac{1}{2}\sigma_1^2t^2 + jm_2t - \frac{1}{2}\sigma_2^2t^2}\\
=&e^{j(m_1+m_2)t - \frac{\sigma_1^2+\sigma_2^2}{2}t^2}
\end{align}

\end{preview}

\begin{preview}
\setcounter{equation}{0}%
\((\xi, \eta)\)
\end{preview}

\begin{preview}
\setcounter{equation}{0}%
\begin{align}
  f(x, y) = \frac{1}{2\pi \sigma_1 \sigma_2 \sqrt{1 - r^2}} \exp\{-\frac{1}{2(1-r^2)}[\frac{(x-m_1)^2}{\sigma_1^2} - \\2r \frac{(x-m_1)(y-m_2)}{\sigma_1 \sigma_2} + \frac{(y - m_2)^2}{\sigma_2^2}]\}, (x, y) \in \mathbb{R}^2
\end{align}

\end{preview}

\begin{preview}
\setcounter{equation}{0}%
\(m_1, m_2, \sigma_1 > 0, \sigma_2 > 0\)
\end{preview}

\begin{preview}
\setcounter{equation}{0}%
\(\vert r \vert < 1\)
\end{preview}

\begin{preview}
\setcounter{equation}{0}%
\((\xi, \eta)\)
\end{preview}

\begin{preview}
\setcounter{equation}{0}%
\((\xi, \eta) \sim N(m_1, \sigma_1^2; m_2, \sigma_2^2;r)\)
\end{preview}

\begin{preview}
\setcounter{equation}{0}%
\(\xi \sim N(m_1, \sigma_1^2), \eta \sim N(m_2, \sigma_2^2).\)
\end{preview}

\begin{preview}
\setcounter{equation}{0}%
\(E(\xi) = m_1, D(\xi) = \sigma_1^2;\)
\end{preview}

\begin{preview}
\setcounter{equation}{0}%
\(E(\eta) = m_2, D(\eta) = \sigma_2^2;\)
\end{preview}

\begin{preview}
\setcounter{equation}{0}%
\(Cov(\xi, \eta) = r \sigma_1 \sigma_2, \rho_{\xi\eta} = r.\)
\end{preview}

\begin{preview}
\setcounter{equation}{0}%
\((\xi, \eta)\)
\end{preview}

\begin{preview}
\setcounter{equation}{0}%
\(r = 0\)
\end{preview}

\begin{preview}
\setcounter{equation}{0}%
\(\xi\)
\end{preview}

\begin{preview}
\setcounter{equation}{0}%
\(\eta\)
\end{preview}

\begin{preview}
\setcounter{equation}{0}%
\(\xi\)
\end{preview}

\begin{preview}
\setcounter{equation}{0}%
\(\eta\)
\end{preview}

\begin{preview}
\setcounter{equation}{0}%
\(f(x, y) = f_\xi(x) f_\eta(y) \Leftrightarrow r = 0.\)
\end{preview}

\begin{preview}
\setcounter{equation}{0}%
\begin{align}
E
\begin{bmatrix}
\xi \\ \eta
\end{bmatrix}
=
\begin{bmatrix}
E(\xi)\\ E(\eta)
\end{bmatrix}
=
\begin{bmatrix}
m_1 \\ m_2
\end{bmatrix}
= M
\end{align}

\end{preview}

\begin{preview}
\setcounter{equation}{0}%
\begin{align}
  \Sigma =
\begin{bmatrix}
\sigma_1^2&r\sigma_1\sigma_2\\
r\sigma_1\sigma_2&\sigma_2^2
\end{bmatrix}
\end{align}

\end{preview}

\begin{preview}
\setcounter{equation}{0}%
\(\sigma_1 > 0, \sigma_2 > 0, \vert r \vert < 1\)
\end{preview}

\begin{preview}
\setcounter{equation}{0}%
\(\vert \Sigma \vert \neq 0\)
\end{preview}

\begin{preview}
\setcounter{equation}{0}%
\begin{align}
  X=
\begin{bmatrix}
x\\y
\end{bmatrix}
\end{align}

\end{preview}

\begin{preview}
\setcounter{equation}{0}%
\begin{align}
  f(x, y) =& \frac{1}{2\pi \sigma_1 \sigma_2 \sqrt{1 - r^2}} \exp\{-\frac{1}{2(1-r^2)}[\frac{(x-m_1)^2}{\sigma_1^2} - \\
&2r \frac{(x-m_1)(y-m_2)}{\sigma_1 \sigma_2} + \frac{(y - m_2)^2}{\sigma_2^2}]\}, (x, y) \in \mathbb{R}^2\\
=&\frac{1}{2\pi\vert\Sigma\vert^{1/2}}\exp\{-\frac{1}{2}(X - M)' \Sigma^{-1} (X-M)\}
\end{align}

\end{preview}

\begin{preview}
\setcounter{equation}{0}%
\((\xi, \eta) \sim N(M, \Sigma).\)
\end{preview}

\begin{preview}
\setcounter{equation}{0}%
\((\xi_1, \xi_2, ..., \xi_n)\)
\end{preview}

\begin{preview}
\setcounter{equation}{0}%
\(f(x_1, x_2, ..., x_n) = \frac{1}{(2\pi)^{n/2}\vert\Sigma\vert^{1/2}}\exp\{-\frac{1}{2}(X-M)'\Sigma^{-1}(X-M)\}\)
\end{preview}

\begin{preview}
\setcounter{equation}{0}%
\(\Sigma = (\sigma_{ij})\)
\end{preview}

\begin{preview}
\setcounter{equation}{0}%
\(\vert \Sigma \vert\)
\end{preview}

\begin{preview}
\setcounter{equation}{0}%
\(X = (x_1, x_2, ..., x_n)'\)
\end{preview}

\begin{preview}
\setcounter{equation}{0}%
\( M=(m_1, m_2, ..., m_n)'\)
\end{preview}

\begin{preview}
\setcounter{equation}{0}%
\((\xi_1, \xi_2, ..., \xi_n)\)
\end{preview}

\begin{preview}
\setcounter{equation}{0}%
\(X = (X_1, X_2, ..., X_n)^\top\)
\end{preview}

\begin{preview}
\setcounter{equation}{0}%
\begin{align}
  \varphi(t) = \exp\{jM^\top t-\frac{1}{2}t^\top C t\}\label{con:Characteristic}
\end{align}

\end{preview}

\begin{preview}
\setcounter{equation}{0}%
\(t = (t_1, t_2, ..., t_m)^\top , M = E(X) = (m_1, m_2, ..., m_n)^\top\)
\end{preview}

\begin{preview}
\setcounter{equation}{0}%
\(\ref{con:Characteristic}\)
\end{preview}

\begin{preview}
\setcounter{equation}{0}%
\(\varphi(u)\)
\end{preview}

\begin{preview}
\setcounter{equation}{0}%
\(\vert C \vert = 0\)
\end{preview}

\begin{preview}
\setcounter{equation}{0}%
\(\omega \rightarrow (X(\omega, t), t \in (-\infty, +\infty))\)
\end{preview}

\begin{preview}
\setcounter{equation}{0}%
\(\{X_t, t \in R\}\)
\end{preview}

\begin{preview}
\setcounter{equation}{0}%
\((\Omega, F, P)\)
\end{preview}

\begin{preview}
\setcounter{equation}{0}%
\(T\subset R\)
\end{preview}

\begin{preview}
\setcounter{equation}{0}%
\(t \in T, X_t(\omega)\)
\end{preview}

\begin{preview}
\setcounter{equation}{0}%
\begin{align}
\{X_t(\omega), t\in T\}
\end{align}

\end{preview}

\begin{preview}
\setcounter{equation}{0}%
\((\Omega, F, P)\)
\end{preview}

\begin{preview}
\setcounter{equation}{0}%
\begin{align}
\{X_t(\omega), t\in T\} = (X_1, X_2, \cdots, X_n)
\end{align}

\end{preview}

\begin{preview}
\setcounter{equation}{0}%
\begin{align}
\{X_t(\omega), t\in T\} = (X_1, X_2, \cdots, X_n, \cdots)
\end{align}

\end{preview}

\begin{preview}
\setcounter{equation}{0}%
\(T=[0, +\infty)\)
\end{preview}

\begin{preview}
\setcounter{equation}{0}%
\begin{align}
\{X_t(\omega), t \in T\} = \{X_t(\omega), t \in [0, +\infty)\}
\end{align}

\end{preview}

\begin{preview}
\setcounter{equation}{0}%
\(T = \{(x, y): a < x < b, c < y < d\}\)
\end{preview}

\begin{preview}
\setcounter{equation}{0}%
\begin{align}
\{X_t(\omega), t \in T\}
\end{align}

\end{preview}

\begin{preview}
\setcounter{equation}{0}%
\(X_t, t \in T\)
\end{preview}

\begin{preview}
\setcounter{equation}{0}%
\(\{X_t, t \in T\}\)
\end{preview}

\begin{preview}
\setcounter{equation}{0}%
\(T \times \Omega = \{(t, \omega): t\in T, \omega \in \Omega\}\)
\end{preview}

\begin{preview}
\setcounter{equation}{0}%
\(T\)
\end{preview}

\begin{preview}
\setcounter{equation}{0}%
\(X_t(\omega)\)
\end{preview}

\begin{preview}
\setcounter{equation}{0}%
\(T \times \Omega\)
\end{preview}

\begin{preview}
\setcounter{equation}{0}%
\(t \in T, X_t(\omega)\)
\end{preview}

\begin{preview}
\setcounter{equation}{0}%
\((\Omega, F, P)\)
\end{preview}

\begin{preview}
\setcounter{equation}{0}%
\(\omega_0 \in \Omega\)
\end{preview}

\begin{preview}
\setcounter{equation}{0}%
\(x_t(\omega_0)\)
\end{preview}

\begin{preview}
\setcounter{equation}{0}%
\(\{X_t(\omega), t \in T\}\)
\end{preview}

\begin{preview}
\setcounter{equation}{0}%
\(\{X_t, t \in T\}\)
\end{preview}

\begin{preview}
\setcounter{equation}{0}%
\(\{\varphi_{t_1, t_2, ..., t_n}(u_1, u_2, ..., t_n): t_i \in T, i = 1, 2, 3,..., n, (u_1, u_2, ..., u_n) \in R^n, n \geq 1\}\)
\end{preview}

\begin{preview}
\setcounter{equation}{0}%
\(\{X_t(\rightarrow), t\in T\}\)
\end{preview}

\begin{preview}
\setcounter{equation}{0}%
\(\varphi_{t_1, t_2,...,t_n}(u_1, u_2, ..., u_n) = E(e^{j(u_1X_{t_1}+u_2X_{t_2}+...+u_nX_{tn})})\)
\end{preview}

\begin{preview}
\setcounter{equation}{0}%
\((X_{t_1}, X_{t_2}, \cdots, X_{t_n})\)
\end{preview}

\begin{preview}
\setcounter{equation}{0}%
\(\{X_t(\omega), t \in T\}\)
\end{preview}

\begin{preview}
\setcounter{equation}{0}%
\begin{align}
m(t) \hat{=} E(X_t) = \int^{+\infty}_{-\infty} x \mathrm{d} F_t(x), t\in T
\end{align}

\end{preview}

\begin{preview}
\setcounter{equation}{0}%
\(D(t) \hat{=} D[X_t] = E[X_t - m(t)]^2\)
\end{preview}

\begin{preview}
\setcounter{equation}{0}%
\(\{X_t(\rightarrow), t \in T\}\)
\end{preview}

\begin{preview}
\setcounter{equation}{0}%
\(\sigma(t) = \sqrt{D_X(t)}\)
\end{preview}

\begin{preview}
\setcounter{equation}{0}%
\begin{align}
C(s, t) \hat{=} Cov(X_s, X_t) = E\{[X_s - m(s)][X_t - m(t)]\}
\end{align}

\end{preview}

\begin{preview}
\setcounter{equation}{0}%
\begin{align}
  R(s, t) \hat{=} E[X_sX_t]
\end{align}

\end{preview}

\begin{preview}
\setcounter{equation}{0}%
\(\{X_t, t \in T\}\)
\end{preview}

\begin{preview}
\setcounter{equation}{0}%
\(\{Y_t, t \in T\}\)
\end{preview}

\begin{preview}
\setcounter{equation}{0}%
\begin{align}
  Z_t \hat{=} X_t + jY_t, t \in T, j = \sqrt{-1}
\end{align}

\end{preview}

\begin{preview}
\setcounter{equation}{0}%
\begin{align}
m_Z(t) \hat{=}E[X_t] + jE[Y_t], t \in T.
\end{align}

\end{preview}

\begin{preview}
\setcounter{equation}{0}%
\begin{align}
  D_Z(t) \hat{=} E\{\vert Z_t - m_Z(t)\vert^2\} = D_X(t) + D_Y(t).
\end{align}

\end{preview}

\begin{preview}
\setcounter{equation}{0}%
\begin{align}
  R_Z(s, t) \hat= E[Z_S \bar{Z_t}].
\end{align}

\end{preview}

\begin{preview}
\setcounter{equation}{0}%
\((\Omega, F, P)\)
\end{preview}

\begin{preview}
\setcounter{equation}{0}%
\(T\)
\end{preview}

\begin{preview}
\setcounter{equation}{0}%
\(t \in T\)
\end{preview}

\begin{preview}
\setcounter{equation}{0}%
\((\Omega, F, P)\)
\end{preview}

\begin{preview}
\setcounter{equation}{0}%
\((X_t^{(1)}(\rightarrow),X_t^{(2)}(\rightarrow),...,X_t^{(n)}(\rightarrow))\)
\end{preview}

\begin{preview}
\setcounter{equation}{0}%
\begin{align}
  \{(X_t^{(1)}(\rightarrow),X_t^{(2)}(\rightarrow),...,X_t^{(n)}(\rightarrow)), t\in T\}
\end{align}

\end{preview}

\end{document}
